
$\int \frac{2 e^{2 x}-e^x}{\sqrt{3 e^{2 x}-6 e^x-1}} d x=\int \frac{\left(2 e^x-1\right) e^x}{\sqrt{3\left(e^{2 x}-2 e^x-\frac{1}{3}\right)}} d x=\int \frac{\left(2 e^x-1\right) e^x}{\sqrt{3} \sqrt{e^{2 x}-2 e^x-\frac{1}{3}}} d x$
$\frac{1}{\sqrt{3}} \int \frac{\frac{2}{\sqrt{3}} \sec \theta \tan \theta}{\sqrt{\frac{4}{3} \sec ^2 \theta-\frac{4}{3}}} d \theta=\frac{2}{3} \int \frac{\sec \theta \tan \theta}{\sqrt{\frac{4}{3}\left(\sec ^2 \theta-1\right)}}=\frac{2}{3} \int \frac{(\sec \theta \tan \theta)}{\frac{2}{\sqrt{3}} \sqrt{\tan ^2 \theta}} d \theta$
